Primitive_Matchers/IpAddresses_Normalize.thy
@@ -1,7 +1,5 @@
 theory IpAddresses_Normalize
 imports Common_Primitive_Matcher
-        "../Bitmagic/Numberwang_Ln" (*ipv4addr_of_dotdecimal_dotdecimal_of_ipv4addr, we should move this lemma?*)
-        "../Bitmagic/CIDRSplit"
         "Primitive_Normalization"
 begin
 
@@ -36,29 +34,8 @@ subsection{*Normalizing IP Addresses*}
   
 
 
-  definition ipt_ipv4range_negation_type_to_br_intersect :: "ipt_ipv4range negation_type list \<Rightarrow> 32 wordinterval" where
-    "ipt_ipv4range_negation_type_to_br_intersect l = l2br_negation_type_intersect (NegPos_map ipt_ipv4range_to_intervall l)" 
 
-  lemma ipt_ipv4range_negation_type_to_br_intersect: "wordinterval_to_set (ipt_ipv4range_negation_type_to_br_intersect l) =
-      (\<Inter> ip \<in> set (getPos l). ipv4s_to_set ip) - (\<Union> ip \<in> set (getNeg l). ipv4s_to_set ip)"
-    apply(simp add: ipt_ipv4range_negation_type_to_br_intersect_def l2br_negation_type_intersect NegPos_map_simps)
-    using ipt_ipv4range_to_intervall by blast
-
-
-  definition br_2_cidr_ipt_ipv4range_list :: "32 wordinterval \<Rightarrow> ipt_ipv4range list" where
-    "br_2_cidr_ipt_ipv4range_list r = map (\<lambda> (base, len). Ip4AddrNetmask (dotdecimal_of_ipv4addr base) len) (ipv4range_split r)"
-
-
-  lemma br_2_cidr_ipt_ipv4range_list: "(\<Union> ip \<in> set (br_2_cidr_ipt_ipv4range_list r). ipv4s_to_set ip) = wordinterval_to_set r"
-    proof -
-    (*have Union_rule: "\<And>P Q S. \<forall>a. P a = Q a \<Longrightarrow> (\<Union>a\<in>S. P a) = (\<Union>x\<in>S. Q x)" by presburger*)
-    have "\<And>a. ipv4s_to_set (case a of (base, x) \<Rightarrow> Ip4AddrNetmask (dotdecimal_of_ipv4addr base) x) = (case a of (x, xa) \<Rightarrow> ipv4range_set_from_bitmask x xa)"
-      by(clarsimp simp add: ipv4addr_of_dotdecimal_dotdecimal_of_ipv4addr)
-    hence "(\<Union> ip \<in> set (br_2_cidr_ipt_ipv4range_list r). ipv4s_to_set ip) = \<Union>((\<lambda>(x, y). ipv4range_set_from_bitmask x y) ` set (ipv4range_split r))"
-      unfolding br_2_cidr_ipt_ipv4range_list_def by(simp)
-    thus ?thesis
-    using ipv4range_split_bitmask by presburger
-  qed
+  
 
 
 
