Simple_Firewall/SimpleFw_Semantics.thy
@@ -1,10 +1,10 @@
 theory SimpleFw_Semantics
-imports Main "../Bitmagic/IPv4Addr" "../Bitmagic/WordInterval_Lists" "../Semantics_Ternary/Negation_Type"
+imports Main "../Semantics_Ternary/Negation_Type"
   "../Firewall_Common_Decision_State"
+  "../Primitive_Matchers/IpAddresses"
   "../Primitive_Matchers/Iface"
   "../Primitive_Matchers/Protocol"
   "../Primitive_Matchers/Simple_Packet"
-  "../Bitmagic/Numberwang_Ln"
 begin
 
 
@@ -125,57 +125,6 @@ subsection{*Simple Ports*}
     by blast
 
 subsection{*Simple IPs*}
-  fun simple_ips_conjunct :: "(ipv4addr \<times> nat) \<Rightarrow> (ipv4addr \<times> nat) \<Rightarrow> (ipv4addr \<times> nat) option" where 
-    "simple_ips_conjunct (base1, m1) (base2, m2) = (if ipv4range_set_from_bitmask base1 m1 \<inter> ipv4range_set_from_bitmask base2 m2 = {}
-       then
-        None
-       else if 
-        ipv4range_set_from_bitmask base1 m1 \<subseteq> ipv4range_set_from_bitmask base2 m2
-       then 
-        Some (base1, m1)
-       else
-        Some (base2, m2)
-      )"
-  
-  lemma simple_ips_conjunct_correct: "(case simple_ips_conjunct (b1, m1) (b2, m2) of Some (bx, mx) \<Rightarrow> ipv4range_set_from_bitmask bx mx | None \<Rightarrow> {}) = 
-      (ipv4range_set_from_bitmask b1 m1) \<inter> (ipv4range_set_from_bitmask b2 m2)"
-    apply(simp split: split_if_asm)
-    using ipv4range_bitmask_intersect by fast
-  declare simple_ips_conjunct.simps[simp del]
-
-  fun ipv4_cidr_tuple_to_intervall :: "(ipv4addr \<times> nat) \<Rightarrow> 32 wordinterval" where
-    "ipv4_cidr_tuple_to_intervall (pre, len) = (
-      let netmask = (mask len) << (32 - len);
-          network_prefix = (pre AND netmask)
-      in ipv4range_range network_prefix (network_prefix OR (NOT netmask))
-     )"
-  declare ipv4_cidr_tuple_to_intervall.simps[simp del]
-
-  lemma ipv4range_to_set_ipv4_cidr_tuple_to_intervall: "ipv4range_to_set (ipv4_cidr_tuple_to_intervall (b, m)) = ipv4range_set_from_bitmask b m"
-    unfolding ipv4_cidr_tuple_to_intervall.simps
-    apply(simp add: ipv4range_set_from_bitmask_alt)
-    by (metis helper3 ipv4range_range_set_eq maskshift_eq_not_mask word_bw_comms(2) word_not_not)
-
-  lemma [code_unfold]: 
-  "simple_ips_conjunct ips1 ips2 = (if ipv4range_empty (ipv4range_intersection (ipv4_cidr_tuple_to_intervall ips1) (ipv4_cidr_tuple_to_intervall ips2))
-       then
-        None
-       else if 
-        ipv4range_subset (ipv4_cidr_tuple_to_intervall ips1) (ipv4_cidr_tuple_to_intervall ips2)
-       then 
-        Some ips1
-       else
-        Some ips2
-      )"
-  apply(simp)
-  apply(cases ips1, cases ips2, rename_tac b1 m1 b2 m2, simp)
-  apply(safe)
-     apply(simp_all add: ipv4range_to_set_ipv4_cidr_tuple_to_intervall simple_ips_conjunct.simps split:split_if_asm)
-    apply fast+
-  done
-  value "simple_ips_conjunct (0,0) (8,1)" (*with the code_unfold lema before, this works!*)
-
-
   lemma simple_match_ip_conjunct: "simple_match_ip ip1 p_ip \<and> simple_match_ip ip2 p_ip \<longleftrightarrow> 
          (case simple_ips_conjunct ip1 ip2 of None \<Rightarrow> False | Some ipx \<Rightarrow> simple_match_ip ipx p_ip)"
   proof -
@@ -192,7 +141,6 @@ subsection{*Simple IPs*}
          (case simple_ips_conjunct (b1, m1) (b2, m2) of None \<Rightarrow> False | Some ipx \<Rightarrow> simple_match_ip ipx p_ip)" .
    } thus ?thesis by(cases ip1, cases ip2, simp)
   qed
-
 
 
 declare simple_matches.simps[simp del]
